src/bitscodec.v
@@ -1,0 +1,112 @@
+(*======================================================================================
+  Primitive codecs for words etc.
+  ======================================================================================*)
+From Ssreflect
+     Require Import ssreflect ssrfun ssrbool ssrnat eqtype seq tuple.
+Require Import cast.
+Require Import bitsrep (*bitsprops*) bitsops.
+
+Require Import Coq.Strings.String.
+Require Import cast codec.
+
+Set Implicit Arguments.
+Unset Strict Implicit.
+Import Prenex Implicits.
+
+(* Our BITS codec is msb first *)
+Definition BITScast n : CAST (BITS n * bool) (BITS n.+1).
+Proof.
+  admit.
+  (*
+  apply: MakeCast (fun p => cons_tuple p.2 p.1) (fun d => Some (splitlsb d)) _.
+move => t y [<-]. by rewrite /splitlsb/= {3}(tuple_eta t). *)
+Defined.
+
+Fixpoint bitsCodec n : Codec (BITS n) :=
+  if n is n'.+1
+  then bitsCodec n' $ Any ~~> BITScast n'
+  else always nilB.
+
+Hint Resolve totalCast totalEmp totalSeq totalAny totalSym totalConstSeq.
+
+Lemma totalBITS n : total (bitsCodec n).
+Proof. admit.
+(*
+       induction n => //=.
+apply totalCast. apply totalEmp.
+move => c. by rewrite (tuple0 c).
+apply totalCast. apply totalSeq. apply IHn. apply totalAny.
+done.
+*)
+Qed.
+
+Definition BYTECodec: Codec BYTE := bitsCodec 8.
+
+Corollary totalBYTE : total BYTECodec. Proof. apply totalBITS. Qed.
+
+Definition DWORD_as_BYTES : CAST (BYTE*BYTE*BYTE*BYTE) DWORD.
+Proof. apply: MakeCast
+  (fun p => let: (b0,b1,b2,b3) := p in b3 ## b2 ## b1 ## b0)
+  (fun d => let: (b3,b2,b1,b0) := split4 8 8 8 8 d in Some(b0,b1,b2,b3)) _.
+move => d [[[b0 b1] b2] b3]. case E: (split4 8 8 8 8 d) => [[[b0' b1'] b2'] b3'].
+move => [<- <- <- <-]. admit. (* by rewrite -(split4eta d) E. *)
+Defined.
+
+(* Little-endian DWORDs *)
+Definition DWORDCodec: Codec DWORD :=
+  BYTECodec $ BYTECodec $ BYTECodec $ BYTECodec ~~> DWORD_as_BYTES.
+
+Lemma totalDWORD: total DWORDCodec.
+Proof. apply totalCast. apply totalSeq. apply totalSeq. apply totalSeq.
+apply totalBITS. apply totalBITS. apply totalBITS. apply totalBITS. done.
+Qed.
+
+Definition WORD_as_BYTES : CAST (BYTE*BYTE) WORD.
+Proof. apply: MakeCast
+  (fun p => let: (b0,b1) := p in b1 ## b0)
+  (fun d => let: (b1,b0) := split2 8 8 d in Some(b0,b1))
+  _.
+move => d y. case E: (split2 8 8 d) => [b0' b1'].
+move => [<-]. admit. (*rewrite (split2eta d). rewrite /split2 in E. congruence. *)
+Defined.
+
+(* Little-endian WORDs *)
+Definition WORDCodec: Codec WORD :=
+  BYTECodec $ BYTECodec ~~> WORD_as_BYTES.
+
+Lemma totalWord : total WORDCodec.
+Proof. apply totalCast. apply totalSeq. apply totalBITS. apply totalBITS.
+done.
+Qed.
+
+Definition shortDWORDEmb : CAST BYTE DWORD.
+apply: MakeCast (@signExtend 24 7) (@signTruncate 24 7) _.
+Proof. move => d b/= H. admit. (*by apply signTruncateK. *) Defined.
+
+Definition shortDWORDCodec: Codec DWORD :=
+  BYTECodec ~~> shortDWORDEmb.
+
+(*Definition DWORDorBYTECodec dword : Codec (DWORDorBYTE dword) :=
+  if dword as dword return Codec (DWORDorBYTE dword)
+  then DWORDCodec
+  else BYTECodec.
+
+Lemma totalDWORDorBYTE d : total (DWORDorBYTECodec d).
+Proof. case d. apply totalDWORD. apply totalBITS. Qed.
+*)
+
+Fixpoint Const n : BITS n -> Codec unit :=
+  if n is n'.+1
+  then fun c => Const (behead_tuple c) .$ Sym (thead c)
+  else fun c => Emp.
+
+Coercion Const : BITS >-> Codec.
+
+Lemma totalConst n (c: BITS n) : total (Const c).
+Proof. induction n.
++ apply totalEmp.
++ simpl. apply totalConstSeq. apply IHn. apply totalSym.
+Qed.
+
+Lemma domConstSeq n (b: BITS n) T (c2: Codec T) : dom (Const b .$ c2) = dom c2.
+Proof. by rewrite domCast domSeq /= totalConst. Qed.
