src/codec.v
@@ -1,0 +1,1209 @@
+From Ssreflect
+     Require Import ssreflect ssrfun ssrbool ssrnat eqtype seq.
+Require Import cast.
+Require Import Coq.Strings.String.
+Require Import Coq.Setoids.Setoid Coq.Classes.Morphisms Coq.Classes.RelationClasses.
+Require Import Coq.Logic.FunctionalExtensionality.
+
+Set Implicit Arguments.
+Unset Strict Implicit.
+Import Prenex Implicits.
+
+(*======================================================================================
+  Concrete syntax for *partial* two-way codecs
+  (partial in the sense that they only encode a subset of values)
+
+  This is very similar to the Rocksalt grammar type, except that Map is generalized to
+  use CASTs so that we can *encode* values as well as decode them.
+
+  Other possibilities
+  - n-ary Alt, with Void just sugar for Alt nil
+  - n-ary Seq, with Emp just sugar for Seq nil (but consider types)
+  ======================================================================================*)
+Definition sym := bool.
+
+Inductive Codec : Type -> Type :=
+| Any : Codec sym
+| Sym :> sym -> Codec unit
+| Emp : Codec unit
+| Void T : Codec T
+| Seq T U (c: Codec T) (d: Codec U) : Codec (T*U)
+(*| Dep (T:finType) F (c: Codec T) (d: forall x:T, Codec (F x)) : Codec {x:T & F x}*)
+| Alt T : Codec T -> Codec T -> Codec T
+| Star T : Codec T -> Codec (seq T)
+| Cast T U: CAST T U -> Codec T -> Codec U
+.
+
+(* Some nice syntax *)
+Notation "x $ y"   := (Seq x y)   (left associativity, at level 42).
+Notation "x ~~> f" := (Cast f x)  (left associativity, at level 50).
+Notation "x ||| y" := (Alt x y)   (at level 55).
+
+
+Notation "x .$ y" := (Seq x y ~~> sndUnitCast _) (at level 30).
+Notation "x $. y" := (Seq x y ~~> fstUnitCast _) (at level 30).
+
+(* Constant parser *)
+Definition always (t: eqType) x : Codec t :=
+    Emp ~~> unConst x.
+
+(* Use one bit to dispatch to left or right summand *)
+Definition SumCond T U (c: Codec T) (d: Codec U) : Codec (T+U) :=
+    Sym false .$ c ~~> unInl _ _
+||| Sym true  .$ d ~~> unInr _ _.
+
+(* Codec for sigma type whose first component is a boolean *)
+Definition DepCond F (c: forall x:bool, Codec (F x)) : Codec {x:bool & F x}:=
+    SumCond (c false) (c true) ~~> sumCast F.
+
+(* Non-dependent conditional *)
+Definition Cond X (c:bool->Codec X) : Codec X :=
+    Sym false .$ c false
+||| Sym true  .$ c true.
+
+(*
+Definition SimpleDep (T:finType) U (c: Codec T) (d: T -> Codec U) : Codec (T*U) :=
+  Dep c d ~~> existTcast T U.
+*)
+
+(* Example of a non-prefix but uniquely-decodeable codec *)
+Example nonprefix : Codec bool :=
+    Sym false             ~~> unConst false
+||| Sym false .$ Sym false ~~> unConst true.
+
+(* We define the interpretation by a fixpoint rather than an inductive family because
+   inversion has trouble with the latter when it is GADT-style *)
+Fixpoint interps t interp (l: seq sym) (xs: seq t) : Prop :=
+  if xs is x::xs'
+  then exists s l1 l2, l = s::(l1++l2) /\ interp (s::l1) x /\ interps interp l2 xs'
+  else l = nil.
+
+Fixpoint interp t (c: Codec t){struct c} : seq sym -> t -> Prop :=
+match c in Codec t return seq sym -> t -> Prop with
+| Any          => fun l b => l = b::nil
+| Emp          => fun l _ => l = nil
+| Sym b        => fun l _ => l = b::nil
+| Void _       => fun l _ => False
+| Cast T U f c => fun l v => exists w, v = upcast f w /\ interp c l w
+| Alt _ c d    => fun l v => interp c l v \/ interp d l v
+| Seq _ _ c d  => fun l v => exists l1 l2, l = l1++l2 /\ interp c l1 v.1 /\ interp d l2 v.2
+(*| Dep _ _ c d  => fun l v => let: existT x w := v in
+                             exists l1 l2, l = l1++l2 /\ interp c l1 x /\ interp (d x) l2 w*)
+| Star T c     => fun l v => interps (interp c) l v
+end.
+
+(* This is the inductive version
+Inductive interp : forall t, Codec t -> seq sym -> t -> Prop :=
+| interp_Any b : @interp sym Any [::b] b
+| interp_Emp : interp Emp nil tt
+| interp_Sym b : interp (Sym b) [::b] tt
+| interp_Cast T U f c w l : interp c l w -> interp (@Cast T U f c) l (upcast f w)
+| interp_Alt1 T c d l v : interp c l v -> interp (@Alt T c d) l v
+| interp_Alt2 T c d l v : interp d l v -> interp (@Alt T c d) l v
+| interp_Seq T U c d l1 l2 v1 v2 : interp c l1 v1 -> interp d l2 v2 -> interp (@Seq T U c d) (l1++l2) (v1,v2)
+| interp_StarNil T (c:Codec T) : interp (Star c) nil nil
+| interp_StarCons T (c:Codec T) s l1 l2 x xs : interp c (s::l1) x -> interp (Star c) l2 xs -> interp (Star c) (s::(l1++l2)) (x::xs)
+.
+*)
+
+(* Simplification lemms for interpretation *)
+Lemma interpAny l b : interp Any l b <-> l = [::b].
+Proof. done. Qed.
+
+Lemma interpEmp l   : interp Emp l tt <-> l = nil.
+Proof. done. Qed.
+
+Lemma interpSym b l : interp (Sym b) l tt <-> l = [::b].
+Proof. done. Qed.
+
+Lemma interpVoid t l (x:t) : interp (Void _) l x <-> False.
+Proof. done. Qed.
+
+Lemma interpAlt t (c1 c2: Codec t) (l: seq sym) x:
+  interp (Alt c1 c2) l x <-> interp c1 l x \/ interp c2 l x.
+Proof. done. Qed.
+
+Lemma interpSeq t1 t2 (c1: Codec t1) (c2: Codec t2) l x:
+  interp (Seq c1 c2) l x <-> exists l1 l2, l = l1++l2 /\ interp c1 l1 x.1 /\ interp c2 l2 x.2.
+Proof. done. Qed.
+
+Lemma interpSeqSym t (c: Codec t) s (l: seq sym) x:
+  interp (Seq (Sym s) c) l (tt,x) <-> exists l', l = s::l' /\ interp c l' x.
+Proof. rewrite interpSeq /=.
+split. move => [l1 [l2 [H1 [H2 H3]]]]. subst. firstorder.
+move => [l' [H1 H2]]. subst. exists [::s]. exists l'. split => //.
+Qed.
+
+Lemma interpCast t u (c: Codec t) (f: CAST t u) l v:
+  interp (Cast f c) l v <-> exists w, v = upcast f w /\ interp c l w.
+Proof. split => H. destruct H as [w H]. by exists w.
+destruct H as [w [H1 H2]]. subst. firstorder. Qed.
+
+Lemma interpStar t (c: Codec t) (l: seq sym) xs :
+  interp (Star c) l xs <->
+  match l, xs with s::l', x::xs' =>
+    (exists l1 l2, l' = l1++l2 /\ interp c (s::l1) x /\ interp (Star c) l2 xs')
+  | nil, nil => True
+  | _, _ => False
+  end.
+Proof. induction xs. destruct l => //.
+split => //.
+destruct l => //. by move => [s [l1 [l2 [H1 H2]]]].
+simpl. move => [s' [l1 [l2 [H1 [H2 H3]]]]]. inversion H1. subst.
+exists l1, l2. firstorder.
+destruct l => //. move => [l1 [l2 [H1 [H2 H3]]]]. subst.
+simpl. exists s, l1, l2. firstorder.
+Qed.
+
+Hint Rewrite interpAny interpEmp interpSym interpVoid interpAlt
+             interpSeqSym interpSeq interpCast interpStar : interp.
+
+(*======================================================================================
+  Size analysis
+  ======================================================================================*)
+Fixpoint maxSize t (c:Codec t) : option nat :=
+match c with
+| Any     => Some 1
+| Emp     => Some 0
+| Sym b  => Some 1
+| Void _ => Some 0
+| Alt _ c d => if maxSize c is Some x then if maxSize d is Some y then Some (maxn x y) else None else None
+| Seq t1 t2 c d =>
+  if maxSize c is Some x then if maxSize d is Some y then Some (x + y) else None else None
+(*| Dep t1 t2 c1 c2 =>
+  let xs := Finite.mixin_enum (Finite.class t1) in
+  foldr (fun x n => max (maxSize (c2 x)) n) (maxSize c1) xs*)
+| Cast _ _ g c => maxSize c
+| Star _ _ => None
+end.
+
+Definition finiteCodec t (c: Codec t) := maxSize c <> None.
+
+Lemma finiteCodecSeq t u (c: Codec t) (d: Codec u) :
+  finiteCodec (c $ d) <-> finiteCodec c /\ finiteCodec d.
+Proof. rewrite /finiteCodec/=.
+destruct (maxSize c) => //. destruct (maxSize d) => //. intuition. intuition.
+Qed.
+
+Lemma finiteCodecAlt t (c d: Codec t) :
+  finiteCodec (c ||| d) <-> finiteCodec c /\ finiteCodec d.
+Proof. rewrite /finiteCodec/=.
+destruct (maxSize c) => //. destruct (maxSize d) => //. intuition. intuition.
+Qed.
+
+Lemma finiteCodecCast t u (c: Codec t) (f: CAST t u):
+  finiteCodec (c ~~> f) <-> finiteCodec c.
+Proof. by rewrite /finiteCodec/=. Qed.
+
+Fixpoint minSize t (c:Codec t) : nat :=
+match c with
+| Any     => 1
+| Emp     => 0
+| Sym b  => 1
+| Void _ => 0
+| Alt _ c d => minn (minSize c) (minSize d)
+| Seq t1 t2 c1 c2 => minSize c1 + minSize c2
+(*| Dep t1 t2 c1 c2 =>
+  let xs := Finite.mixin_enum (Finite.class t1) in
+  foldr (fun x n => min (minSize (c2 x)) n) (minSize c1) xs*)
+| Cast _ _ g c => minSize c
+| Star _ _ => 0
+end.
+
+Lemma minSizeSound t (c: Codec t) : forall l x, interp c l x -> size l >= minSize c.
+Proof. induction c => l x /=H.
+- by subst. - by subst. - by subst. - done.
+- elim H => [l1 [l2 [-> [H2 H3]]]].
+  specialize (IHc1 _ _ H2).
+  specialize (IHc2 _ _ H3).
+  rewrite size_cat. apply leq_add => //.
+- elim H => H'.
+  specialize (IHc1 _ _ H'). by rewrite geq_min IHc1.
+  specialize (IHc2 _ _ H'). by rewrite geq_min IHc2 orbT.
+- done.
+- elim H => [w [H1 H2]]. apply: IHc H2.
+Qed.
+
+Lemma maxSizeSound t (c: Codec t) :
+  forall n, maxSize c = Some n -> forall l x, interp c l x -> size l <= n.
+Proof. induction c => n /=EQ l x /=H.
+- injection EQ => <-. by subst.
+- injection EQ => <-. by subst.
+- by subst.
+- done.
+- elim H => [l1 [l2 [-> [H2 H3]]]].
+  case E1: (maxSize c1) => [n1 |]; rewrite E1 in EQ => //.
+  case E2: (maxSize c2) => [n2 |]; rewrite E2 in EQ => //.
+  specialize (IHc1 _ E1 _ _ H2).
+  specialize (IHc2 _ E2 _ _ H3).
+  rewrite size_cat.
+  injection EQ => <-. apply leq_add => //.
+- case E1: (maxSize c1) => [n1 |]; rewrite E1 in EQ => //.
+  case E2: (maxSize c2) => [n2 |]; rewrite E2 in EQ => //.
+  elim H => H'.
+  * specialize (IHc1 _ E1 _ _ H'). injection EQ => <-. by rewrite leq_max IHc1.
+  * specialize (IHc2 _ E2 _ _ H'). injection EQ => <-. by rewrite leq_max IHc2 orbT.
+- done.
+- elim H => [w [H1 H2]]. apply: IHc H2 => //.
+Qed.
+
+Fixpoint consSize m ms :=
+  if ms is n::ms' then
+    if m < n then m::ms
+    else if m == n then ms
+    else n::consSize m ms' else [::m].
+
+Fixpoint unionSizes (ms ns : seq nat) :=
+  if ms is n::ms' then unionSizes ms' (consSize n ns) else ns.
+
+Fixpoint addToSizes m ns :=
+  if ns is n::ns' then m+n::addToSizes m ns' else nil.
+
+Fixpoint addSizes ms ns :=
+  if ms is m::ms' then unionSizes (addSizes ms' ns) (addToSizes m ns) else nil.
+
+Fixpoint sizes t (c:Codec t) : seq nat :=
+match c with
+| Any     => [::1]
+| Emp     => [::0]
+| Sym b  => [::1]
+| Void _ => [::0]
+| Alt _ c d => unionSizes (sizes c) (sizes d)
+| Seq t1 t2 c d => addSizes (sizes c) (sizes d)
+| Cast _ _ g c => sizes c
+| Star _ _ => nil
+end.
+
+Require Import Ssreflect.div.
+(* Compute minimum, maximum, and gcd of number of bits *)
+Definition stats t (c: Codec t) :=
+  let s := sizes c
+  in (head 0 s, last 0 s, foldr gcdn 0 s).
+
+Lemma consSizeMem x xs : forall y, x \in xs -> x \in consSize y xs.
+Proof. induction xs => // => x' MEM/=.
+case (x' < a). rewrite in_cons. by rewrite MEM orbT.
+case (x' == a) => //. rewrite in_cons. apply/orP. rewrite in_cons in MEM.
+case/orP: MEM => H1. by left. right. by apply IHxs.
+Qed.
+
+Lemma consSizeMemHead x xs : x \in consSize x xs.
+Proof. induction xs => //=. by rewrite in_cons eq_refl.
+case (x < a). by rewrite in_cons eq_refl.
+case E: (x == a). rewrite (eqP E). by rewrite in_cons eq_refl.
+rewrite in_cons. apply/orP. by right.
+Qed.
+
+Lemma unionSizesMemR x xs : forall ys, x \in ys -> x \in unionSizes xs ys.
+Proof. induction xs => //=. move => ys MEM. apply IHxs. destruct ys => //.
+by apply consSizeMem. Qed.
+
+Lemma unionSizesMemL x xs: forall ys, x \in xs -> x \in unionSizes xs ys.
+Proof. induction xs => //= ys. rewrite in_cons.
+case/orP. move/eqP ->. apply unionSizesMemR. apply consSizeMemHead. apply IHxs. Qed.
+
+Lemma addToSizesMem a y ys : y \in ys -> a+y \in addToSizes a ys.
+Proof. induction ys => //= H.
+rewrite in_cons in H.
+case/orP: H => H'.
+rewrite (eqP H'). by rewrite mem_head.
+rewrite in_cons.
+apply/orP. right. by apply IHys.
+Qed.
+
+Lemma addSizesMem (x y:nat) xs: forall ys, x \in xs -> y \in ys -> x+y \in addSizes xs ys.
+Proof. induction xs => //= ys.
+rewrite in_cons. case/orP.
+move/eqP => ->. move => H1. apply unionSizesMemR. by apply addToSizesMem.
+move => Hx Hy. apply unionSizesMemL. by apply IHxs.
+Qed.
+
+Lemma sizesSound t (c: Codec t) :
+  finiteCodec c ->
+  forall l x, interp c l x -> size l \in sizes c.
+Proof. induction c => FIN /= l x /=H.
+- by subst.
+- by subst.
+- by subst.
+- done.
+- elim H => [l1 [l2 [-> [H2 H3]]]].
+  apply finiteCodecSeq in FIN. elim FIN => [FIN1 FIN2].
+  specialize (IHc1 FIN1 _ _ H2).
+  specialize (IHc2 FIN2 _ _ H3).
+  rewrite size_cat.
+  by apply addSizesMem.
+- apply finiteCodecAlt in FIN. elim FIN => [FIN1 FIN2].
+  elim H => H'.
+  * specialize (IHc1 FIN1 _ _ H'). by apply unionSizesMemL.
+  * specialize (IHc2 FIN2 _ _ H'). by apply unionSizesMemR.
+- by rewrite /finiteCodec in FIN.
+- elim H => {H} [w [H1 H2]].
+  apply finiteCodecCast in FIN.
+  apply: IHc H2 => //.
+Qed.
+
+Lemma sizesProp t (c: Codec t) P :
+  finiteCodec c ->
+  all P (sizes c) ->
+  forall l x, interp c l x -> P (size l).
+Proof. move => FIN ALL l x I.
+       set n := size l.
+       have SS:= sizesSound FIN I.
+       admit.
+       (*apply: allP.  apply ALL. done. Qed. *)
+       Qed.
+
+(*======================================================================================
+  Semantic equivalence of codecs
+  ======================================================================================*)
+Definition codecEq t (c1 c2: Codec t) := forall l x, interp c1 l x <-> interp c2 l x.
+Notation "x '===' y" := (codecEq x y) (at level 70, no associativity).
+
+(* It's an equivalence relation *)
+Global Instance codecEqEqu t : Equivalence (@codecEq t).
+Proof. constructor; red; rewrite /codecEq.
++ done.
++ firstorder.
++ move => c1 c2 c3 H1 H2 l x. specialize (H1 l x). specialize (H2 l x). firstorder.
+Qed.
+
+(* It's preserved by constructors *)
+Global Instance codecEq_seq_m t u:
+  Proper (@codecEq t ==> @codecEq u ==> @codecEq _) (@Seq t u).
+Proof. move => p1 p2 EQ1 q1 q2 EQ2 .
+move => l [x y].
+autorewrite with interp. split => /= H /=. destruct H as [l1 [l2 [H1 [H2 H3]]]].
+exists l1, l2. rewrite /codecEq in EQ1, EQ2. firstorder.
+destruct H as [l1 [l2 [H1 [H2 H3]]]].
+exists l1, l2. rewrite /codecEq in EQ1, EQ2. firstorder.
+Qed.
+
+Global Instance codecEq_alt_m t:
+  Proper (@codecEq t ==> @codecEq t ==> @codecEq _) (@Alt t).
+Proof. move => p1 p2 EQ1 q1 q2 EQ2 .
+move => l x.
+autorewrite with interp. split => /= H /=. rewrite /codecEq in EQ1, EQ2. firstorder.
+rewrite /codecEq in EQ1, EQ2. firstorder.
+Qed.
+
+Global Instance codecEq_cast_m t u:
+  Proper (eq ==> @codecEq _ ==> @codecEq _) (@Cast t u).
+Proof. move => p1 p2 EQ1 q1 q2 EQ2.
+move => l x. autorewrite with interp.
+split => /= H /=.
+destruct H as [w [H1 H2]]. exists w. subst. firstorder.
+destruct H as [w [H1 H2]]. exists w. subst. firstorder.
+Qed.
+
+Global Instance codecEq_interp_m t: Proper (@codecEq t ==> eq ==> eq ==> iff) (@interp t).
+Proof. move => r1 r2 EQ l1 l2 -> x1 x2 ->.
+rewrite /codecEq in EQ. firstorder.
+Qed.
+
+
+(* Commutativity, associativity, idempotence and unit for Alt *)
+Lemma AltC t (c d: Codec t) : c ||| d === d ||| c.
+Proof. move => l x. autorewrite with interp. split => /= H; intuition. Qed.
+
+Lemma AltA t (c d e: Codec t) : c ||| d ||| e === c ||| (d ||| e).
+Proof. move => l x. autorewrite with interp. split => /= H; intuition. Qed.
+
+Lemma AltN t (c d e: Codec t) : c ||| c === c.
+Proof. move => l x. autorewrite with interp. split => /= H; intuition. Qed.
+
+Lemma AltVoid t (c: Codec t) : c ||| Void _ === c.
+Proof. move => l x. autorewrite with interp. split => /= H; intuition. Qed.
+
+Lemma VoidAlt t (c: Codec t) : Void _ ||| c === c.
+Proof. move => l x. autorewrite with interp. split => /= H; intuition. Qed.
+
+(* Push cast into Alt *)
+Lemma CastAlt t u (f: CAST t u) (c: Codec t) (d: Codec t) :
+  (c ||| d) ~~> f === (c ~~> f) ||| (d ~~> f).
+Proof. move => l x. autorewrite with interp. split => /= H; destruct H; firstorder. Qed.
+
+(* Composition of casts *)
+Lemma ComposeCast t u v (f:CAST t u) (g: CAST u v) (c: Codec t):
+  c ~~> f ~~> g === c ~~> composeCast f g.
+Proof. move => l x. autorewrite with interp. split => /= H.
++ destruct H as [w [H1 [w' [H2 H3]]]]. subst. by exists w'.
++ destruct H as [w [H1 H2]]. subst. exists (f w). firstorder.
+Qed.
+
+(* Elimination of cast by Void *)
+Lemma CastVoid t u f:
+  Void t ~~> f === Void u.
+Proof. firstorder. Qed.
+
+(* Pulling casts out of Seq *)
+Lemma CastSeq t u v (f:CAST t v) (c: Codec t) (d: Codec u) :
+  (c ~~> f) $ d === (c $ d) ~~> pairOfCasts f (idCast _).
+Proof. move => l [x y]. autorewrite with interp. split => /= H.
+destruct H as [l1 [l2 [H1 [H2 H3]]]]. destruct H2 as [w [H4 H5]]. subst.
+exists (w, y). firstorder.
+destruct H as [[a b] [H1 [l1 [l2 [H2 [H3 H4]]]]]]. subst. simpl in H1, H3, H4.
+injection H1 => [-> ->]. exists l1, l2. firstorder.
+Qed.
+
+Lemma SeqCast t u v (f:CAST u v) (c: Codec t) (d: Codec u) :
+  c $ (d ~~> f) === (c $ d) ~~> pairOfCasts (idCast _) f.
+Proof. move => l [x y]. autorewrite with interp. split => /= H.
+destruct H as [l1 [l2 [H1 [H2 H3]]]]. destruct H3 as [w [H4 H5]]. subst.
+exists (x, w). firstorder.
+destruct H as [[a b] [H1 [l1 [l2 [H2 [H3 H4]]]]]]. subst. simpl in H1, H3, H4.
+injection H1 => [-> ->]. exists l1, l2. firstorder.
+Qed.
+
+(* Common prefix under Alt *)
+Lemma SeqAlt t u (b:Codec u) (c d: Codec t):
+  b $ (c ||| d) === b $ c ||| b $ d.
+Proof. move => l x. autorewrite with interp. firstorder. Qed.
+
+(* Common postfix under Alt *)
+Lemma AltSeq t u (b:Codec u) (c d: Codec t):
+  (c ||| d) $ b === c $ b ||| d $ b.
+Proof. move => l x. autorewrite with interp. firstorder. Qed.
+
+(* Special case for .$ *)
+Lemma CastConstSeq t u (c: Codec _) (d: Codec t) (f: CAST t u) :
+  c .$ d ~~> f ===  c .$ (d ~~> f).
+Proof. move => l x. autorewrite with interp.
+split => /= H. destruct H as [w [EQ H]]. autorewrite with interp in H.
+destruct H as [w' [EQ' H]]. autorewrite with interp in H.
+destruct H as [l1 [l2 [H1 [H2 H3]]]].
+exists (tt,x). split => //.
+autorewrite with interp. exists l1, l2. split => //. split => //. subst. simpl.
+destruct w' as [u' w']. simpl in H2.
+destruct u'. done.
+autorewrite with interp. exists w. split => //. by  subst.
+
+destruct H as [w [EQ H]]. autorewrite with interp in H.
+destruct H as [l1 [l2 [H1 [H2 H3]]]].
+autorewrite with interp in H3. destruct H3 as [w' [H3 H4]]. subst.
+exists w'. split => //. autorewrite with interp. exists (tt,w'). split => //.
+autorewrite with interp. exists l1, l2. split => //.
+split => //. simpl. by destruct w as [[] w].
+Qed.
+
+Lemma SeqEmp t (c: Codec t) :
+  c $ Emp === c ~~> unitRcast _.
+Proof. move => l [x []]. autorewrite with interp. split.
++ move => [l1 [l2 [H1 [H2 H3]]]]. exists x. simpl in H3. subst. rewrite cats0. firstorder.
++ move => [w [H1 H2]]. simpl in H1. injection H1 => [->]. exists l, nil. firstorder.
+Qed.
+
+Lemma EmpSeq t (c: Codec t) :
+  c ~~> unitLcast _ === Emp $ c.
+Proof. move => l [[] x]. autorewrite with interp. split.
++ move => [w [H1 H2]]. simpl in H1. injection H1 => [->]. exists nil, l. firstorder.
++ move => [l1 [l2 [H1 [H2 H3]]]]. exists x. simpl in H2. subst. firstorder.
+Qed.
+
+Lemma SeqAssoc t1 t2 t3 (c1: Codec t1) (c2: Codec t2) (c3: Codec t3) :
+  c1 $ c2 $ c3 === c1 $ (c2 $ c3) ~~> pairAssocCast _ _ _.
+Proof. move => l. move => [[x y] z]. autorewrite with interp. split.
++ move => [l1 [l2 [H1 [H2 H3]]]]. subst. exists (x,(y,z)).
+  destruct H2 as [l3 [l4 [H4 [H5 H6]]]]. subst. rewrite -catA.
+  split => //. exists l3, (l4++ l2). firstorder.
++ move => [w [H1 H2]]. simpl in H2. destruct H2 as [l1 [l2 [H3 [H4 H5]]]]. subst.
+  destruct H5 as [l3 [l4 [H6 [H7 H8]]]]. subst. exists (l1++l3),l4. rewrite catA.
+  split => //. injection H1 => [-> -> ->]. firstorder.
+Qed.
+
+Lemma VoidSeq t u (c: Codec t) : Void u $ c === Void _.
+Proof. firstorder. Qed.
+
+Lemma SeqVoid t u (c: Codec t) : c $ Void u === Void _.
+Proof. firstorder. Qed.
+
+(*======================================================================================
+  Smart constructors
+  ======================================================================================*)
+Fixpoint cSeq t1 t2 (r1:Codec t1) (r2:Codec t2) : Codec (t1*t2) :=
+match r1 in Codec t1, r2 in Codec t2 return Codec (t1*t2) with
+| _, Void _ => Void _
+| Void _, _ => Void _
+| Cast _ _ f r1, r2 => cSeq r1 r2 ~~> pairOfCasts f (idCast _)
+| Emp, r2 => r2 ~~> unitLcast _
+| r1, Emp => r1 ~~> unitRcast _
+| Seq _ _ r1a r1b, r2 => cSeq r1a (cSeq r1b r2) ~~> pairAssocCast _ _ _
+| r1, r2 => Seq r1 r2
+end.
+
+Lemma cSeqSound t (c: Codec t) : forall u (d: Codec u), cSeq c d === Seq c d.
+Proof.
+induction c => u d.
++ destruct d => //=. by rewrite SeqEmp. by rewrite SeqVoid.
++ destruct d => //=. by rewrite SeqEmp. by rewrite SeqVoid.
++ rewrite <-EmpSeq. destruct d => //=. by rewrite CastVoid.
++ rewrite VoidSeq. by destruct d => //=.
++ destruct d => //=. by rewrite SeqAssoc -IHc2 -IHc1.
+  by rewrite SeqAssoc -IHc2 -IHc1.
+  by rewrite SeqEmp. by rewrite SeqVoid.
+  by rewrite SeqAssoc -IHc2 -IHc1.
+  by rewrite SeqAssoc -IHc2 -IHc1.
+  by rewrite SeqAssoc -IHc2 -IHc1.
+  by rewrite SeqAssoc -IHc2 -IHc1.
++ destruct d => //=. by rewrite SeqEmp. by rewrite SeqVoid.
++ destruct d => //=. by rewrite SeqEmp. by rewrite SeqVoid.
++ rewrite CastSeq -IHc. destruct d => //=. rewrite IHc. by rewrite SeqVoid CastVoid.
+Qed.
+
+Fixpoint cAltAux t (r1 r2: Codec t) : Codec t :=
+match r1, r2 with
+(*
+| r1, Void _ => r1
+*)
+| Void _, r2 => r2
+| Alt _ r1a r1b, _ => Alt r1a (cAltAux r1b r2)
+| r1, r2 => Alt r1 r2
+end.
+
+Lemma cVoidAltSound t (c:Codec t): cAltAux (Void _) c === c.
+Proof. by destruct c. Qed.
+
+Lemma cAltAuxSound t c : forall d: Codec t, cAltAux c d === Alt c d.
+Proof. induction c => //. move => d. by rewrite cVoidAltSound VoidAlt.
+move => d. rewrite AltA. rewrite <- IHc2. destruct d => //.
+Qed.
+
+Definition simplCast t (c: Codec t) :=
+match c with
+| Cast _ _ f (Void _) => Void _
+| Cast _ _ f (Cast _ _ g (Void _)) => Void _
+| _ => c
+end.
+
+Lemma simplCastSound t (c: Codec t) : simplCast c === c.
+Proof. destruct c => //=. destruct c0 => //=. rewrite CastVoid => //.
+destruct c1 => //=. rewrite CastVoid => //. rewrite CastVoid => //.
+Qed.
+
+Definition cAlt t (r1 r2: Codec t) := cAltAux (simplCast r1) (simplCast r2).
+
+Lemma cAltSound t (c d: Codec t): cAlt c d === Alt c d.
+Proof. rewrite /cAlt. by rewrite cAltAuxSound 2!simplCastSound. Qed.
+
+Fixpoint cCast t (c: Codec t) : forall u, CAST t u -> Codec u :=
+match c in Codec t return forall u, CAST t u -> Codec u with
+| Cast t' u' g c => fun _ f => cCast c (composeCast g f)
+| c => fun _ f => Cast f c
+end.
+
+Lemma cCastSound t (c: Codec t) : forall u (f: CAST t u), cCast c f === Cast f c.
+Proof. induction c => // u f. by rewrite /= IHc ComposeCast. Qed.
+
+(* Deterministic language *)
+Definition detInterp t (c: Codec t) :=
+  forall l v w, interp c l v -> interp c l w -> v=w.
+
+(* Prefix-free language *)
+Definition prefixFreeInterp t (c: Codec t) :=
+  forall l e v w, interp c l v -> interp c (l++e) w -> e=nil.
+
+(* Deterministic *and* prefix-free *)
+Definition dpfInterp t (c: Codec t) :=
+  forall l e v w, interp c l v -> interp c (l++e) w -> v=w /\ e=nil.
+
+(*======================================================================================
+  Executable encoder function
+  ======================================================================================*)
+(* Note that we insist that encoding a value in a starred codec actually produces a
+non-empty list *)
+Fixpoint encs t enc (xs: seq t) : option (seq sym) :=
+  if xs is x::xs'
+  then if enc x is Some (b::bs) then
+       if encs enc xs' is Some bs'
+       then Some(b::bs++bs') else None else None
+  else Some nil.
+
+Definition encShortest := true.
+
+Fixpoint enc t (c:Codec t) : t -> option (seq sym) :=
+match c with
+| Any => fun b => Some (b::nil)
+| Emp => fun _ => Some nil
+| Sym b => fun _ => Some (b::nil)
+| Void _ => fun _ => None
+| Cast _ _ f c => fun x =>
+  if downcast f x is Some y then enc c y else None
+| Seq _ _ c d => fun x =>
+  let: (y,z) := x in
+  if enc c y is Some bs1 then
+  if enc d z is Some bs2 then Some (bs1++bs2)
+  else None else None
+| Alt _ c d => fun x =>
+  match enc c x, enc d x with
+  | Some bs1, Some bs2 =>
+    if size bs1 < size bs2 then Some bs1 else Some bs2
+  | None, Some bs2 => Some bs2
+  | Some bs1, None => Some bs1
+  | None, None => None
+  end
+| Star _ c => fun x => encs (enc c) x
+end.
+
+Lemma encsSound t (c: Codec t) : (forall v l, enc c v = Some l -> interp c l v) ->
+  (forall vs l, encs (enc c) vs = Some l -> interps (interp c) l vs).
+Proof. move => H. induction vs => l.
++ destruct l => //.
++ simpl.
+  case E1: (enc c a) => [l1 |] => //. specialize (H _ _ E1).
+  case E2: (encs (enc c) vs) => [l2 |] => //.  specialize (IHvs _ E2).
+  destruct l1 => //. move => [<-].
+  exists s, l1, l2. firstorder.
+  destruct l1 => //.
+Qed.
+
+Lemma encSound t (c: Codec t) : forall v l, enc c v = Some l -> interp c l v.
+Proof.
+  admit.
+  (*
+  induction c => v l [/=EQ] /=; autorewrite with interp => /=.
+(* Any *)
+done.
+(* Sym *)
+destruct v. subst. constructor.
+(* Emp *)
+destruct v. subst. constructor.
+(* Void *)
+done.
+(* Seq *)
+destruct v as [v1 v2].
+case E1: (enc c1 v1) => [l1 |]; rewrite E1 in EQ => //.
+case E2: (enc c2 v2) => [l2 |]; rewrite E2 in EQ => //.
+exists l1, l2. injection EQ => [<-]. split => //. intuition.
+(*(* Dep *)
+destruct v as [x w].
+case E1: (enc c x) => [l1 |]; rewrite E1 in EQ => //.
+case E2: (enc (d x) w) => [l2 |]; rewrite E2 in EQ => //.
+exists l1, l2. injection EQ => [<-]. split => //. intuition. *)
+(* Alt *)
+case E1: (enc c1 v) => [l1 |]; rewrite E1 in EQ => //.
+case E2: (enc c2 v) => [l2 |]; rewrite E2 in EQ => //.
+case B: (size l1 < size l2); rewrite B in EQ;
+injection EQ => [<-]; intuition.
+injection EQ => [<-]; intuition.
+case E2: (enc c2 v) => [l2 |]; rewrite E2 in EQ => //.
+injection EQ => [<-]; intuition.
+(* Star *)
+apply encsSound => //.
+(* Cast *)
+case E: (downcast c v) => [v' |]; rewrite E in EQ => //.
+exists v'. have IV := castinv E. intuition.
+*)
+Qed.
+
+
+(*======================================================================================
+  Domain and totality, based on encoding
+  ======================================================================================*)
+Definition dom t (c: Codec t) : pred t := SimplPred (fun x => isSome (enc c x)).
+Definition total t (c: Codec t) := dom c =1 predT.
+
+Lemma domEmp : dom Emp = predT. Proof. done. Qed.
+Lemma domAny : dom Any = predT. Proof. done. Qed.
+Lemma domSym b : dom (Sym b) = predT. Proof. done. Qed.
+Lemma domVoid t : dom (Void t) = [pred _ | false]. Proof. done. Qed.
+Lemma domAlt T (c1 c2: Codec T) : dom (c1 ||| c2) = predU (dom c1) (dom c2).
+Proof. apply functional_extensionality => x. rewrite /dom/=.
+destruct (enc c1 x) => //. destruct (enc c2 x) => //.
+by destruct (_ < _). destruct (enc c2 x) => //.
+Qed.
+
+Lemma domSeq T U (c: Codec T) (d: Codec U) : dom (c $ d) = [pred x | dom c x.1 && dom d x.2].
+Proof. apply functional_extensionality => x. destruct x as [y z]. simpl.
+rewrite /dom/=. destruct (enc c y) => //. destruct (enc d z) => //. Qed.
+
+Lemma domCast T U (c: Codec T) (f: CAST T U) :
+  dom (c ~~> f) = [pred u | if downcast f u is Some t then dom c t else false].
+Proof. apply functional_extensionality => u.
+rewrite /dom/=.
+destruct (downcast f u) => //.
+Qed.
+
+Lemma totalEmp : total Emp. Proof. done. Qed.
+Lemma totalAny : total Any. Proof. done. Qed.
+Lemma totalSym b : total (Sym b). Proof. done. Qed.
+Lemma totalApp t (c: Codec t) : total c -> forall v, isSome (enc c v). Proof. done. Qed.
+
+Lemma totalCast T U (c: Codec T) (f: CAST T U) : total c -> castIsTotal f -> total (c ~~> f).
+Proof. move => tc tf v. rewrite domCast/=. rewrite /castIsTotal in tf. specialize (tf v).
+destruct (downcast f _) => //. apply tc. Qed.
+
+Lemma totalSeq T U (c: Codec T) (d: Codec U) : total c -> total d -> total (c $ d).
+Proof. move => totalc totald x. by rewrite domSeq /= totalc totald. Qed.
+
+Lemma totalConstSeq T (c: Codec unit) (d: Codec T) : total c -> total d -> total (c .$ d).
+Proof.  move => tc td x. apply totalCast => //. apply totalSeq => //. Qed.
+
+(*======================================================================================
+  Derivatives of codecs
+  ======================================================================================*)
+Fixpoint null t (c: Codec t) : Codec t :=
+match c with
+| Emp => Emp
+| Alt _ c1 c2 => cAlt (null c1) (null c2)
+| Seq _ _ c1 c2 => cSeq (null c1) (null c2)
+| Cast _ _ f c => cCast (null c) f
+| Star _ c => Cast (unNil _) Emp
+| _ => Void _
+end.
+
+Fixpoint valIfNull t (c: Codec t) : option t :=
+match c with
+| Emp => Some tt
+| Void _ => None
+| Alt _ c1 c2 =>
+  if valIfNull c1 is Some x then Some x else valIfNull c2
+| Cast _ _ f c =>
+  if valIfNull c is Some x then Some (upcast f x) else None
+| Seq _ _ c1 c2 =>
+  if valIfNull c1 is Some x1
+  then if valIfNull c2 is Some x2
+  then Some (x1,x2) else None else None
+| Star _ c =>
+  Some nil
+| _ => None
+end.
+
+Fixpoint valsIfNull t (c: Codec t) : seq t :=
+match c with
+| Emp          => [::tt]
+| Void _       => nil
+| Alt _ c1 c2  => valsIfNull c1 ++ valsIfNull c2
+| Cast _ _ f c  => [seq upcast f x | x <- valsIfNull c]
+| Seq _ _ c1 c2 => [seq (x,y) | x <- valsIfNull c1, y <- valsIfNull c2]
+| Star _ c => [::nil]
+| _ => nil
+end.
+
+Fixpoint derivSym t (s: sym) (c: Codec t) : Codec t :=
+match c with
+| Any => Emp ~~> unConst s
+| Sym s' => if s==s' then Emp  else Void _
+| Alt _ c1 c2 => cAlt (derivSym s c1) (derivSym s c2)
+| Seq _ _ c1 c2 => cAlt (cSeq (derivSym s c1) c2) (cSeq (null c1) (derivSym s c2))
+| Cast _ _ f c => cCast (derivSym s c) f
+| Star _ c => cSeq (derivSym s c) (Star c) ~~> unCons _
+| _ => Void _
+end.
+
+Fixpoint interpAll t (r: Codec t) l xs :=
+  if xs is x::xs then interp r l x /\ interpAll r l xs else True.
+
+(* Only one direction *)
+Lemma interpValIfNull t (r: Codec t) : forall x, valIfNull r = Some x -> interp r nil x.
+Proof. induction r => x/=.
++ done.
++ done.
++ done.
++ done.
++ case E1: (valIfNull r1) => [x1 |] => //.
+  case E2: (valIfNull r2) => [x2 |] => //.
+  move => [<-]. exists nil, nil. split => //. split. by apply IHr1. by apply IHr2.
++ case E1: (valIfNull r1) => [x1 |]. move => [<-].
+  have I1 := ((IHr1 _) E1). by left.
+  move => H.
+  have I2 := ((IHr2 _) H). by right.
++ by move => [<-].
++ move => H.
+  case E: (valIfNull r) => [y |]; rewrite E in H => //.
+  injection H => <-. exists y. split => //. by apply IHr.
+Qed.
+
+Lemma interpValIfNullConv t (r: Codec t) : forall x, interp r nil x -> exists y, valIfNull r = Some y.
+Proof. induction r => x/=.
++ done.
++ done.
++ move => _. by exists tt.
++ done.
++ move => [l1 [l2 [H1 [H2 H3]]]]. destruct l1 => //. destruct l2 => //.
+  destruct (IHr1 _ H2) as [y1 H4].
+  destruct (IHr2 _ H3) as [y2 H5]. exists (y1,y2).
+  by rewrite H4 H5.
++ elim => H. destruct (IHr1 _ H) as [y H1]. exists y. by rewrite H1.
+  destruct (IHr2 _ H) as [y H1].
+  case E: (valIfNull r1) => [z |]. by exists z. by exists y.
++ move => H. by exists nil.
++ move => [w [H1 H2]].
+  destruct (IHr _ H2) as [z H3].
+  exists (c z). by rewrite H3.
+Qed.
+
+Corollary interpValIfNullNone t (r: Codec t) x : valIfNull r = None -> interp r nil x -> False.
+Proof.
+move => H1 H2.
+destruct (interpValIfNullConv H2) as [z H3].
+by rewrite H1 in H3.
+Qed.
+
+Lemma interpNull t (r: Codec t) : forall l x, interp (null r) l x <-> (l = nil /\ interp r nil x).
+Proof. induction r => l x; split => //.
++ move => [H1 H2]. done.
++ move => [H1 H2]. done.
++ intuition.
++ intuition.
++ move => /= H.
+  rewrite -> cSeqSound in H. rewrite -> interpSeq in H.
+  destruct H as [l1 [l2 [H1 [H2 H3]]]]. subst.
+  destruct (IHr1 l1 x.1) as [I1a I1b].
+  destruct (IHr2 l2 x.2) as [I2a I2b].
+  specialize (I1a H2). specialize (I2a H3).
+  destruct I1a as [-> I1a]. destruct I2a as [-> I2a]. split => //.  exists nil, nil. intuition.
+  move => [H1 [l1 [l2 [H2 [H3 H4]]]]].
+  simpl. rewrite cSeqSound interpSeq. exists nil, nil. subst. split => //. destruct l1 => //. destruct l2 => //.
+  split => //. apply IHr1; intuition.  apply IHr2; intuition.
++ move => /=H. rewrite -> cAltSound in H. rewrite -> interpAlt in H.
+destruct H.
+- specialize (IHr1 l x). destruct IHr1 as [I1 I2]. specialize (I1 H). intuition.
+- specialize (IHr2 l x). destruct IHr2 as [I1 I2]. specialize (I1 H). intuition.
+  move => [H1 H2]. subst.
+  simpl. rewrite cAltSound interpAlt. destruct H2.
+  specialize (IHr1 nil x). intuition.
+  specialize (IHr2 nil x). intuition.
++ simpl. by move => [_ [-> ->]].
+  move => [-> H]. exists tt. destruct x => //. simpl in H.
+  destruct H as [s [l1 [l2 [H1 H2]]]].  done.
++ simpl. move => H1. rewrite -> cCastSound in H1. rewrite -> interpCast in H1.
+destruct H1 as [w [H1 H2]]. subst.
+destruct (IHr l w) as [I1 _]. specialize (I1 H2). destruct I1 as [-> I1].
+split => //.  exists w. intuition.
+move => [-> [w [H1 H2]]]. simpl. rewrite cCastSound. rewrite interpCast.
+exists w. split => //. apply IHr. intuition.
+Qed.
+
+Lemma interpDerivSym c t (r:Codec t) : forall s x, interp (derivSym c r) s x <-> interp r (c::s) x.
+Proof.
+  admit.
+  (*
+  induction r => l x.     
++ split => //= H. destruct H as [_ [H1 H2]]. by subst.
+  injection H => [-> ->]. exists tt. intuition.
++ split => //= H.
+  case E: (c == s). rewrite (eqP E). rewrite E in H. simpl in H. by subst.
+  rewrite E in H. by simpl in H.
+  admit.
+  (*
+  injection H as [->]. rewrite eq_refl. simpl. congruence.
+  simpl. split => //. *)
++ simpl. done.
++ simpl. admit. (*rewrite cAltSound 2!cSeqSound. rewrite interpAlt 2!interpSeq.
+  split => H.
+  destruct H.
+  - destruct H as [l1 [l2 [H1 [H2 H3]]]]. subst.
+    exists (c::l1). exists l2. split => //. rewrite -> IHr1 in H2. intuition.
+  - destruct H as [l1 [l2 [H1 [H2 H3]]]]. rewrite -> interpNull in H2.
+    destruct H2 as [-> H2]. simpl in H1. subst. rewrite -> IHr2 in H3.
+    exists nil. exists (c::l2). intuition.
+  - destruct H as [l1 [l2 [H1 [H2 H3]]]].
+    destruct l1.
+    simpl in H1.  subst. right. exists nil, l. split => //.
+    rewrite interpNull. intuition. by rewrite IHr2.
+    left. simpl in H1. injection H1 => [H4 H5]. subst. exists l1, l2. split => //.
+    rewrite IHr1. intuition. *)
++ simpl. rewrite cAltSound interpAlt.
+  split => H.
+  - destruct H. admit. (*left. by apply IHr1.
+    right. by apply IHr2. *)
+  - admit. (*destruct H. left. by apply IHr1.
+    right. by apply IHr2. *)
++ simpl. admit. (* split => H. destruct H as [[x' xs] [H1 H2]].
+  rewrite -> cSeqSound in H2. rewrite -> interpSeq in H2.
+  destruct H2 as [l1 [l2 [H3 [H4 H5]]]]. simpl in H4, H5. rewrite -> IHr in H4.
+  subst. simpl. exists c, l1, l2. intuition.
+  destruct x => //.
+  simpl in H.
+  destruct H as [s [l1 [l2 [H1 [H2 H3]]]]].
+  injection H1 => [H4 H5]. subst. exists (t,x). split => //.
+  rewrite cSeqSound. rewrite interpSeq. exists l1, l2. split => //. split.
+  by rewrite IHr. done. *)
++ simpl. split => H.
+  (*
+  rewrite -> cCastSound in H. rewrite -> interpCast in H.
+  destruct H as [w [H1 H2]].  subst. exists w. split => //. by rewrite -> IHr in H2.
+  rewrite cCastSound. rewrite interpCast. destruct H as [w [H1 H2]].
+  exists w. split => //. by rewrite IHr.
+   *)
+  admit. *)
+Qed.
+
+(* Taking derivatives preserves determinism and prefix-free-ness *)
+Lemma dpfInterpDerivSym t (c: Codec t) a : dpfInterp c -> dpfInterp (derivSym a c).
+Proof. rewrite /dpfInterp => H l e v w. rewrite 2!interpDerivSym=> I1 I2. apply: H I1 I2. Qed.
+
+(*======================================================================================
+  Bit reader decoding of codecs
+
+  We use derivatives "on-the-fly" to avoid any backtracking for deterministic codecs.
+  ======================================================================================*)
+(*
+Require Import monad bitreader.
+Fixpoint codecToBitReader bits t (c: Codec t) : BitReader (option t) :=
+  if valIfNull c is Some x then retn (Some x)
+  else if bits isn't bits'.+1 then retn None
+  else
+    let! b = readBit;
+    codecToBitReader bits' (derivSym b c).
+
+(* Soundness of decoding *)
+Lemma codecToBitReaderSound bits : forall t (c: Codec t) cursor cursor' l x rest,
+  runBitReader (codecToBitReader bits c) cursor l = Some(cursor', rest, Some x) ->
+  exists l', l = l' ++ rest /\ interp c l' x.
+Proof. induction bits => t c cursor cursor' l x rest /= H //.
+case E: (valIfNull c) => [y |]; rewrite E/= in H => //.
++ injection H => [<- <-] H'. exists nil. split => //. by apply interpValIfNull.
+case E: (valIfNull c) => [y |]; rewrite E in H => //.
+injection H => [<- ->] H'. have I:= interpValIfNull E. by exists nil.
+destruct l => //. simpl in H.  destruct cursor => //.
+simpl in H. destruct cursor => //. destruct (IHbits _ _ _ cursor' _ _ rest H) as [l' [-> H2]].
+exists (b::l').
+split => //. by apply interpDerivSym.
+Qed.
+
+(* Completeness of decoding: if a value is in the interpretation of a prefix-free codec, then
+   codecToBitReader will return it *)
+Require Import x86proved.bitsrep x86proved.bitsops x86proved.cursor.
+Lemma codecToBitReaderComplete n  : forall t (c: Codec t) cursor cursor' l,
+  dpfInterp c ->
+  size l <= n ->
+  apart (size l) cursor cursor' ->
+  forall x, interp c l x ->
+  forall rest, runBitReader (codecToBitReader n c) cursor (l ++ rest) = Some(cursor', rest, Some x).
+Proof.
+induction n => //.
+
++ move => t c cursor cursor' l DPF SIZE AP x I e. destruct l => //=.
+  case E: (valIfNull c) => [y |].
+- have J := interpValIfNull E. simpl in AP. subst.
+  by elim (DPF _ _ _ _ I J) => [-> _].
+- contradiction (interpValIfNullNone E I).
+
++ move => t c cursor cursor' l DPF SIZE AP x I e.
+  destruct l => //.
+  * (* l = nil *)
+    simpl.
+    case E: (valIfNull c) => [y |]. have J := (interpValIfNull E).
+    simpl in AP. subst. elim (DPF _ _ _ _ I J) => [-> _]. done.
+    contradiction (interpValIfNullNone E I).
++ specialize (IHn _ (derivSym s c)).
+  have DPF': dpfInterp (derivSym s c) by apply dpfInterpDerivSym.
+  simpl (size _) in AP. destruct cursor => //. simpl in AP.
+  subst.
+  specialize (IHn _ _ _ DPF' SIZE AP).
+  simpl.
+  case E: (valIfNull c) => [y |].
+  - simpl. rewrite /dpfInterp in DPF.
+    have HH := interpValIfNull E.
+    rewrite /dpfInterp in DPF. specialize (DPF _ _ _ _ HH I). by destruct DPF.
+  - simpl. apply IHn. by rewrite <-interpDerivSym in I.
+Qed.
+
+Corollary codecToFiniteBitReaderComplete t (c: Codec t) n cursor cursor' :
+  dpfInterp c ->
+  maxSize c = Some n ->
+  forall l x, interp c l x ->
+  apart (size l) cursor cursor' ->
+  forall rest, runBitReader (codecToBitReader n c) cursor (l++rest) = Some(cursor', rest, Some x).
+Proof.
+move => DPF MAX l x I AP rest.
+have SOUND := maxSizeSound MAX I.
+eapply (codecToBitReaderComplete DPF SOUND AP I rest).
+Qed.
+
+Corollary codecToFiniteBitReaderRoundtrip t (c: Codec t) l e x n cursor cursor':
+  dpfInterp c ->
+  maxSize c = Some n ->
+  apart (size l) cursor cursor' ->
+  enc c x = Some l ->
+  runBitReader (codecToBitReader n c) cursor (l ++ e) = Some(cursor', e, Some x).
+Proof. move => DPF MAX AP ENC.
+apply codecToFiniteBitReaderComplete => //. by apply encSound. Qed.
+
+Example ex : Codec bool :=
+    Sym false .$ Sym true  ~~> unConst false
+||| Sym true  .$ Sym false ~~> unConst true.
+
+(*======================================================================================
+  Executable decoder function; assume that all uses of Alt are non-ambiguous
+  ======================================================================================*)
+
+Inductive DecRes T :=
+  DecYes (t: T) (rest: seq sym) | DecNo.
+
+Definition castRes t u (f:CAST t u) (r: DecRes t) :=
+  if r is DecYes v res then DecYes (upcast f v) res else DecNo _.
+
+Fixpoint empRes t (c:Codec t) :DecRes t:=
+  match c with
+  | Emp => DecYes tt nil
+  | Cast _ _ f c => if empRes c is DecYes v r then DecYes (upcast f v) r else DecNo _
+  | _ => DecNo _
+  end.
+
+(* Not structurally recursive
+Fixpoint decs t dec (l: seq sym) : DecRes (seq t) :=
+  if l is s::l'
+  then if dec l is DecYes x l' then if decs _ dec l' is DecYes xs l'' then DecYes (x::xs) l''
+  else DecNo _ else DecNo _
+  else DecYes nil nil.
+*)
+
+(* Note that dec actually does backtracking in Alt case *)
+Implicit Arguments DecNo [T].
+
+Fixpoint dec t (c: Codec t) (l: seq sym) : DecRes t :=
+match c with
+| Any       => if l is b::l then DecYes b l else DecNo
+| Sym b     => if l is b'::l then if b==b'
+               then DecYes tt l else DecNo else DecNo
+| Emp       => DecYes tt l
+| Void _    => DecNo
+| Alt _ c d =>
+  if dec c l is DecYes x l' then DecYes x l'
+  else dec d l
+| Seq _ _ c d =>
+  if dec c l is DecYes x l'
+  then if dec d l' is DecYes y l''
+  then DecYes (x,y) l'' else DecNo else DecNo
+| Cast _ _ f c =>
+  if dec c l is DecYes x l'
+  then DecYes (f x) l' else DecNo
+| Star _ c =>
+  DecNo
+end.
+
+(* Soundness applies regardless of determinism or prefix-free-ness *)
+Lemma decSound t (c: Codec t) :
+  forall l x rest, dec c l = DecYes x rest ->
+  exists l', l = l' ++ rest /\ interp c l' x.
+Proof. induction c => l x rest /= EQ.
+(* Any *)
+case E: l => [| x' xs]; rewrite E in EQ => //.
+injection EQ => [-> ->]. by exists (x::nil).
+(* Sym *)
+case E: l => [| x' xs]; rewrite E in EQ => //.
+case E': (s==x'); rewrite E' in EQ => //.
+exists (x'::nil). rewrite (eqP E'). injection EQ => [<- H']. done.
+(* Emp *)
+exists nil. simpl. injection EQ => [] ->. done.
+(* Void *)
+done.
+(* Seq *)
+destruct x as [x1 x2].
+case E1: (dec c1 l) => [x l' |]; rewrite E1 in EQ => //.
+case E2: (dec c2 l') => [y l'' |]; rewrite E2 in EQ => //.
+injection EQ => [<- <- <-].
+destruct (IHc1 _ _ _ E1) as [l1 [-> H1]].
+destruct (IHc2 _ _ _ E2) as [l2 [-> H2]].
+exists (l1++l2). rewrite catA. split => //. simpl. by exists l1, l2.
+(*(* Dep *)
+case E1: (dec c l) => [x' l' | |]; rewrite E1 in EQ => //.
+case E2: (dec (d x') l') => [y l'' | |]; rewrite E2 in EQ => //.
+injection EQ => [<- <-].
+destruct (IHc _ _ _ E1) as [l1 [-> H1]].
+destruct (H _ _ _ _ E2) as [l2 [-> H2]].
+exists (l1++l2). rewrite catA. split => //. exists l1, l2. split => //. *)
+(* Alt *)
+case E1: (dec c1 l) => [x' l' |]; rewrite E1 in EQ => //.
+destruct (IHc1 _ _ _ E1) as [l1 [-> H1]].
+exists l1. injection EQ => [-> <-]. split => //. by constructor.
+destruct (IHc2 _ _ _ EQ) as [l2 [-> H2]]. exists l2. split => //. intuition.
+(* Star *)
+done.
+(* Cast *)
+case E1: (dec c0 l) => [x' l' |]; rewrite E1 in EQ => //.
+destruct (IHc _ _ _ E1) as [l1 [-> H1]].
+exists l1. injection EQ => [-> <-]. split => //. by exists x'.
+Qed.
+
+Lemma appeqpref t a: forall b c d: seq t, a++b = c++d ->
+  (exists e, a=c++e /\ d=e++b) \/ (exists e, c=a++e /\ b=e++d).
+Proof.
+induction a => b c d /=EQ. subst. right. by exists c.
+destruct c => //. left. simpl. exists (a::a0). intuition.
+injection EQ => H1 H2. subst. specialize (IHa _ _ _ H1).
+destruct IHa.
+- destruct H as [e [E1 E2]]. subst. left. by exists e.
+- destruct H as [e [E1 E2]]. subst. right. by exists e.
+Qed.
+
+(*
+(* Dec is closed under extension of bytes *)
+Lemma decExt t (c: Codec t) :
+  forall l e,
+  (forall x rest, dec c l = DecYes x rest -> dec c (l ++ e) = DecYes x (rest ++ e))
+  /\
+  (dec c l = DecNo _ -> dec c (l ++ e) = DecNo _).
+Proof. induction c => l e; split => /=.
+(* Any *)
+move => x rest /= H.
+case E: l => [| x' xs]; rewrite E in H => //.
+injection H => [-> ->]. intuition.
+destruct l => //=.
+(* Sym *)
+move => [] rest /= H.
+case E: l => [| x' xs]; rewrite E in H => //.
+case E': (s==x'); rewrite E' in H => //. rewrite (eqP E').
+injection H => [<-]. by rewrite /= eq_refl.
+destruct l => //=.
+case E': (s==s0) => //.
+(* Emp *)
+move => [] rest /= H. by injection H => [->].
+(* Void *)
+done. done. done.
+(* Seq *)
+move => [x1 x2] rest /= H.
+case E1: (dec c1 l) => [x l'| |]; rewrite E1 in H => //.
+case E2: (dec c2 l') => [y l'' | |]; rewrite E2 in H => //.
+injection H => [<- <- <-].
+by rewrite (proj1 (IHc1 _ _) _ _ E1) (proj1 (IHc2 _ _) _  _ E2).
+case E1: (dec c1 l) => [x l'| |] => //.
+case E2: (dec c2 l') => [y l'' | |] => //.
+rewrite (proj1 (IHc1 _ _) _ _ E1). by rewrite (proj2 (IHc2 _ _) E2).
+by rewrite (proj2 (IHc1 _ _) E1).
+(*(* Dep *)
+move => v rest /= H'.
+destruct v as [x w].
+case E1: (dec c l) => [x' l'| |]; rewrite E1 in H' => //.
+case E2: (dec (d x') l') => [y l'' | |]; rewrite E2 in H' => //.
+injection H' => [<- <-] H''. subst.
+rewrite (proj1 (IHc _ _) _ _ E1).
+by rewrite (proj1 (H _ _ _) _  _ E2).
+case E1: (dec c l) => [x l'| |] => //.
+case E2: (dec (d x) l') => [y l'' | |] => //.
+rewrite (proj1 (IHc _ _) _ _ E1). by rewrite (proj2 (H _ _ _) E2).
+by rewrite (proj2 (IHc _ _) E1). *)
+(* Alt *)
+move => x rest /= H.
+case E1: (dec c1 l) => [x' l' | |]; rewrite E1 in H => //.
+rewrite (proj1 (IHc1 _ _) _ _ E1). by injection H => [-> <-].
+rewrite (proj1 (IHc2 _ _) _ _ H). by rewrite (proj2 (IHc1 _ _) E1).
+case E1: (dec c1 l) => [x' l' | |] => E2 //.
+by rewrite (proj2 (IHc1 _ _) E1) (proj2 (IHc2 _ _) E2).
+(* Cast *)
+move => x rest /= H.
+case E1: (dec c0 l) => [x' l' | |]; rewrite E1 in H => //.
+rewrite (proj1 (IHc _ _) _ _ E1). by injection H => [-> <-].
+case E1: (dec c0 l) => [x' l' | |] => E2 //.
+by rewrite (proj2 (IHc _ _) E1).
+Qed.
+
+(* Note that the corresponding property does *not* hold of concatentation. e.g.
+   (00|||0) $$ 1 is prefix-free but (00|0) is not.
+*)
+Lemma altDpf t (c d: Codec t): dpfInterp (Alt c d) -> dpfInterp c /\ dpfInterp d.
+Proof.
+rewrite /dpfInterp => H. split => l e v1 v2 I1 I2.
+apply: (H l e v1 v2); by left.
+apply: (H l e v1 v2); by right.
+Qed.
+
+*)
+
+(*
+Fixpoint ddec t (c: Codec t) (l: seq sym) : DecRes t :=
+if l is b::l' then ddec (deriv b c) l'
+else if null c is Emp then DecYes tt nil else DecNo _.
+*)
+*)
